Test/civl/inductive-sequentialization/2PC.bpl
@@ -88,7 +88,7 @@ modifies ReqCH, VoteCH, DecCH, votes, decisions;
     (decisions[0] == COMMIT() ==> (forall i:int :: pid(i) ==> votes[i] == YES())) &&
     (forall i:int :: pidLe(i,k) ==> decisions[i] == decisions[0]);
   DecCH := (lambda i:int :: (lambda d:decision :: if pidGt(i, k) && d == decisions[0] then 1 else 0));
-  PAs := (lambda {:pool "PARTICIPANT2"} pa:PA :: if is#PARTICIPANT2(pa) && pidGt(pid#PARTICIPANT2(pa), k) then 1 else 0);
+  PAs := (lambda {:pool "PARTICIPANT2"} pa:PA :: if pa is PARTICIPANT2 && pidGt(pa->pid, k) then 1 else 0);
   choice := PARTICIPANT2(k+1);
 }
 
@@ -123,7 +123,7 @@ modifies ReqCH, VoteCH, DecCH, votes, decisions;
   assume dec == COMMIT() ==> (forall i:int :: pid(i) ==> votes[i] == YES());
   decisions[0] := dec;
   DecCH := (lambda i:int :: (lambda d:decision :: if pid(i) && d == dec then 1 else 0));
-  PAs := (lambda pa:PA :: if is#PARTICIPANT2(pa) && pid(pid#PARTICIPANT2(pa)) then 1 else 0);
+  PAs := (lambda pa:PA :: if pa is PARTICIPANT2 && pid(pa->pid) then 1 else 0);
 }
 
 procedure {:IS_invariant}{:layer 4}
@@ -141,7 +141,7 @@ modifies ReqCH, VoteCH, DecCH, votes, decisions;
     assume VoteCH[YES()] >= 0 && VoteCH[NO()] >= 0;
     assume VoteCH[YES()] + VoteCH[NO()] <= n;
     assume VoteCH[YES()] == n ==> (forall i:int :: pid(i) ==> votes[i] == YES());
-    PAs := MapAddPA(SingletonPA(COORDINATOR2(0)), (lambda pa:PA :: if is#PARTICIPANT2(pa) && pid(pid#PARTICIPANT2(pa)) then 1 else 0));
+    PAs := MapAddPA(SingletonPA(COORDINATOR2(0)), (lambda pa:PA :: if pa is PARTICIPANT2 && pid(pa->pid) then 1 else 0));
   }
   else
   {
@@ -149,7 +149,7 @@ modifies ReqCH, VoteCH, DecCH, votes, decisions;
     assume dec == COMMIT() ==> (forall i:int :: pid(i) ==> votes[i] == YES());
     decisions[0] := dec;
     DecCH := (lambda i:int :: (lambda d:decision :: if pid(i) && d == dec then 1 else 0));
-    PAs := (lambda pa:PA :: if is#PARTICIPANT2(pa) && pid(pid#PARTICIPANT2(pa)) then 1 else 0);
+    PAs := (lambda pa:PA :: if pa is PARTICIPANT2 && pid(pa->pid) then 1 else 0);
   }
 }
 
@@ -188,7 +188,7 @@ modifies ReqCH, VoteCH, votes;
   assume VoteCH[YES()] >= 0 && VoteCH[NO()] >= 0;
   assume VoteCH[YES()] + VoteCH[NO()] <= n;
   assume VoteCH[YES()] == n ==> (forall i:int :: pid(i) ==> votes[i] == YES());
-  PAs := MapAddPA(SingletonPA(COORDINATOR2(0)), (lambda pa:PA :: if is#PARTICIPANT2(pa) && pid(pid#PARTICIPANT2(pa)) then 1 else 0));
+  PAs := MapAddPA(SingletonPA(COORDINATOR2(0)), (lambda pa:PA :: if pa is PARTICIPANT2 && pid(pa->pid) then 1 else 0));
 }
 
 procedure {:IS_invariant}{:layer 3}
@@ -210,8 +210,8 @@ modifies ReqCH, VoteCH, votes;
     VoteCH[YES()] + VoteCH[NO()] <= k &&
     (VoteCH[YES()] == k ==> (forall i:int :: pidLe(i,k) ==> votes[i] == YES()));
   PAs := MapAddPA(SingletonPA(COORDINATOR2(0)),
-      MapAddPA((lambda pa:PA :: if is#PARTICIPANT2(pa) && pidLe(pid#PARTICIPANT2(pa), k) then 1 else 0),
-               (lambda {:pool "PARTICIPANT1"} pa:PA :: if is#PARTICIPANT1(pa) && pidGt(pid#PARTICIPANT1(pa), k) then 1 else 0)));
+      MapAddPA((lambda pa:PA :: if pa is PARTICIPANT2 && pidLe(pa->pid, k) then 1 else 0),
+               (lambda {:pool "PARTICIPANT1"} pa:PA :: if pa is PARTICIPANT1 && pidGt(pa->pid, k) then 1 else 0)));
   choice := PARTICIPANT1(k+1);
 }
 
@@ -227,7 +227,7 @@ modifies ReqCH;
     {:add_to_pool "INV2", 0}
     Init(pids, ReqCH, VoteCH, DecCH, decisions);
   ReqCH := (lambda i:int :: if pid(i) then 1 else 0);
-  PAs := MapAddPA(SingletonPA(COORDINATOR2(0)), (lambda pa:PA :: if is#PARTICIPANT1(pa) && pid(pid#PARTICIPANT1(pa)) then 1 else 0));
+  PAs := MapAddPA(SingletonPA(COORDINATOR2(0)), (lambda pa:PA :: if pa is PARTICIPANT1 && pid(pa->pid) then 1 else 0));
 }
 
 procedure {:IS_invariant}{:layer 2}
@@ -238,14 +238,14 @@ modifies ReqCH;
   assert Init(pids, ReqCH, VoteCH, DecCH, decisions);
   if (*)
   {
-    PAs := MapAddPA(SingletonPA(COORDINATOR1(0)), (lambda pa:PA :: if is#PARTICIPANT1(pa) && pid(pid#PARTICIPANT1(pa)) then 1 else 0));
+    PAs := MapAddPA(SingletonPA(COORDINATOR1(0)), (lambda pa:PA :: if pa is PARTICIPANT1 && pid(pa->pid) then 1 else 0));
     assume PAs[COORDINATOR1(0)] > 0;
   }
   else
   {
     ReqCH := (lambda i:int :: if pid(i) then 1 else 0);
-    PAs := MapAddPA(SingletonPA(COORDINATOR2(0)), (lambda pa:PA :: if is#PARTICIPANT1(pa) && pid(pid#PARTICIPANT1(pa)) then 1 else 0));
-    assume (forall pa:PA :: PAs[pa] == 0 <== is#COORDINATOR1(pa));
+    PAs := MapAddPA(SingletonPA(COORDINATOR2(0)), (lambda pa:PA :: if pa is PARTICIPANT1 && pid(pa->pid) then 1 else 0));
+    assume (forall pa:PA :: PAs[pa] == 0 <== pa is COORDINATOR1);
     assume PAs[COORDINATOR2(0)] == 1;
   }
 }
@@ -258,7 +258,7 @@ MAIN1 ({:linear_in "pid"} pids:[int]bool)
 returns ({:pending_async "COORDINATOR1","PARTICIPANT1"} PAs:[PA]int)
 {
   assert Init(pids, ReqCH, VoteCH, DecCH, decisions);
-  PAs := MapAddPA(SingletonPA(COORDINATOR1(0)), (lambda pa:PA :: if is#PARTICIPANT1(pa) && pid(pid#PARTICIPANT1(pa)) then 1 else 0));
+  PAs := MapAddPA(SingletonPA(COORDINATOR1(0)), (lambda pa:PA :: if pa is PARTICIPANT1 && pid(pa->pid) then 1 else 0));
 }
 
 procedure {:atomic}{:layer 2,3}
@@ -349,7 +349,7 @@ requires {:layer 1} Init(pids, ReqCH, VoteCH, DecCH, decisions);
   invariant {:layer 1}{:cooperates} true;
   invariant {:layer 1} 1 <= i && i <= n+1;
   invariant {:layer 1} (forall ii:int :: pid(ii) && ii >= i ==> pids'[ii]);
-  invariant {:layer 1} PAs == MapAddPA(SingletonPA(COORDINATOR1(0)), (lambda pa:PA :: if is#PARTICIPANT1(pa) && pid(pid#PARTICIPANT1(pa)) && pid#PARTICIPANT1(pa) < i then 1 else 0));
+  invariant {:layer 1} PAs == MapAddPA(SingletonPA(COORDINATOR1(0)), (lambda pa:PA :: if pa is PARTICIPANT1 && pid(pa->pid) && pa->pid < i then 1 else 0));
   {
     call pid, pids' := linear_transfer(i, pids');
     async call participant1(pid);
